infoflow+crefine: refine arch split
Signed-off-by: Ryan Barry <ryan.barry@unsw.edu.au>

proof/infoflow/refine/ADT_IF_Refine_C.thy
@@ -5,21 +5,8 @@
  *)
 
 theory ADT_IF_Refine_C
-imports ADT_IF_Refine "CRefine.Refine_C"
+imports ArchADT_IF_Refine "CRefine.Refine_C"
 begin
-
-context begin interpretation Arch . (*FIXME: arch_split*)
-
-definition handleInterruptEntry_C_body_if (*:: "(globals myvars, int, l4c_errortype) com"*) where
-"handleInterruptEntry_C_body_if \<equiv> (
-      (\<acute>irq :== CALL getActiveIRQ();;
-       (Guard SignedArithmetic \<lbrace>True\<rbrace>
-         (IF (ucast \<acute>irq :: word32) \<noteq> (ucast ((ucast (-1 :: 16 word)) :: word32)) THEN
-            CALL handleInterrupt(\<acute>irq)
-          FI)));;
-       \<acute>ret__unsigned_long :== scast EXCEPTION_NONE)"
-
-
 
 definition handleSyscall_C_body_if
   where
@@ -92,9 +79,17 @@ definition handleVMFaultEvent_C_body_if
           FI;;
             \<acute>ret__unsigned_long :== scast EXCEPTION_NONE))"
 
-end
 
 context kernel_m begin
+
+definition handleInterruptEntry_C_body_if (*:: "(globals myvars, int, l4c_errortype) com"*) where
+"handleInterruptEntry_C_body_if \<equiv> (
+      (\<acute>irq :== CALL getActiveIRQ();;
+       (Guard SignedArithmetic \<lbrace>True\<rbrace>
+         (IF (ucast \<acute>irq :: obj_ref) \<noteq> (ucast irqInvalid) THEN
+            CALL handleInterrupt(\<acute>irq)
+          FI)));;
+       \<acute>ret__unsigned_long :== scast EXCEPTION_NONE)"
 
 definition
   "callKernel_C_body_if e \<equiv> case e of
@@ -105,14 +100,13 @@ definition
   | VMFaultEvent t \<Rightarrow> (handleVMFaultEvent_C_body_if (vm_fault_type_from_H t))
   | HypervisorEvent t \<Rightarrow> (SKIP ;; \<acute>ret__unsigned_long :== scast EXCEPTION_NONE)"
 
-
 definition
   kernelEntry_C_if (*::
     "bool \<Rightarrow> event \<Rightarrow> user_context \<Rightarrow> (cstate, (bool \<times> user_context)) nondet_monad"*)
   where
   "kernelEntry_C_if (fp :: bool) e tc \<equiv> do
     t \<leftarrow> gets (ksCurThread_' o globals);
-    setArchTCB_C (arch_tcb_C (to_user_context_C tc)) t;
+    setTCBContext_C (to_user_context_C tc) t;
     exec_C \<Gamma> (callKernel_C_body_if e);
     ex \<leftarrow> gets ret__unsigned_long_';
     r \<leftarrow> return (if (ex = scast EXCEPTION_NONE) then Inr () else Inl ex);
@@ -131,52 +125,126 @@ definition
       {(s, b, (tc,s'))|s b tc s' r. ((r,tc),s') \<in> fst (split (kernelEntry_C_if fp e) s) \<and>
                    b = (case r of Inl x \<Rightarrow> True | Inr x \<Rightarrow> False)}"
 
+definition
+  checkActiveIRQ_C_if :: "user_context \<Rightarrow> (cstate, irq option \<times> user_context) nondet_monad"
+  where
+  "checkActiveIRQ_C_if tc \<equiv>
+   do
+      getActiveIRQ_C;
+      irq \<leftarrow>  gets ret__unsigned_long_';
+      return (if irq = ucast irqInvalid then None else Some (ucast irq), tc)
+   od"
 
-lemma handleInterrupt_ccorres:
-  "ccorres (K dc \<currency> dc) (liftxf errstate id (K ()) ret__unsigned_long_')
-           (invs')
-           (UNIV)
-           []
-           (handleEvent Interrupt)
-           (handleInterruptEntry_C_body_if)"
-proof -
-  have ucast_not_helper_cheating_unsigned:
-    "\<And>a. ucast (a::10 word) \<noteq> (0xFFFF :: word16) \<Longrightarrow> ucast a \<noteq> (0xFFFF::32 word)"
-    by (word_bitwise)
-  show ?thesis
-  apply (rule ccorres_guard_imp2)
-   apply (simp add: handleEvent_def minus_one_norm handleInterruptEntry_C_body_if_def)
-   apply (clarsimp simp: liftE_def bind_assoc)
-   apply (rule ccorres_rhs_assoc)
-   apply (ctac (no_vcg) add: getActiveIRQ_ccorres)
-    apply (rule ccorres_Guard_Seq)
-    apply (rule_tac P="rv \<noteq> Some 0xFFFF" in ccorres_gen_asm)
-    apply wpc
-     apply (simp add: ccorres_cond_empty_iff)
-     apply (rule_tac P=\<top> and P'=UNIV in ccorres_from_vcg)
-     apply (rule allI, rule conseqPre, vcg)
-     apply (clarsimp simp: return_def)
-    apply (clarsimp simp: ucast_not_helper_cheating_unsigned ucast_helper_simps_32
-      ucast_not_helper ccorres_cond_univ_iff ucast_ucast_a is_down)
-    apply (ctac (no_vcg) add: handleInterrupt_ccorres)
-     apply (rule_tac P=\<top> and P'=UNIV in ccorres_from_vcg)
-     apply (rule allI, rule conseqPre, vcg)
-     apply (clarsimp simp: return_def)
+definition
+  check_active_irq_C_if
+  where
+  "check_active_irq_C_if \<equiv> {((tc, s), irq, (tc', s')). ((irq, tc'), s') \<in> fst (checkActiveIRQ_C_if tc s)}"
+
+lemma corres_select_f':
+  "\<lbrakk> \<And>s s'. P s \<Longrightarrow> P' s' \<Longrightarrow> \<forall>s' \<in> fst S'. \<exists>s \<in> fst S. rvr s s'; nf' \<Longrightarrow> \<not> snd S' \<rbrakk>
+      \<Longrightarrow> corres_underlying sr nf nf' rvr P P' (select_f S) (select_f S')"
+  by (clarsimp simp: select_f_def corres_underlying_def)
+
+lemma cur_thread_of_absKState[simp]:
+   "cur_thread (absKState s) = (ksCurThread s)"
+   by (clarsimp simp: cstate_relation_def Let_def absKState_def cstate_to_H_def)
+
+lemma absKState_crelation:
+  "\<lbrakk> cstate_relation s (globals s'); invs' s \<rbrakk> \<Longrightarrow>  cstate_to_A s' = absKState s"
+  apply (clarsimp simp add: cstate_to_H_correct invs'_def cstate_to_A_def)
+  apply (clarsimp simp: absKState_def absExst_def observable_memory_def)
+  apply (case_tac s)
+  apply clarsimp
+  apply (case_tac ksMachineState)
+  apply clarsimp
+  apply (rule ext)
+  by (clarsimp simp: option_to_0_def user_mem'_def pointerInUserData_def ko_wp_at'_def
+                     obj_at'_def typ_at'_def ps_clear_def
+              split: if_splits)
+
+definition
+  handlePreemption_C_if :: "user_context \<Rightarrow> (cstate,user_context) nondet_monad" where
+  "handlePreemption_C_if tc \<equiv> do (exec_C \<Gamma> handleInterruptEntry_C_body_if); return tc od"
+
+lemma handlePreemption_if_def2:
+  "handlePreemption_if tc = do
+     r \<leftarrow> handleEvent Interrupt;
+          stateAssert (\<lambda>s. (ksDomainTime s = 0 \<longrightarrow> ksSchedulerAction s = ChooseNewThread) \<and>
+                            valid_domain_list' s) [];
+          return tc
+   od"
+  apply (clarsimp simp add: handlePreemption_if_def handleEvent_def liftE_def
+                   bind_assoc)
+  apply (rule bind_eqI)
+  apply (rule ext)
+  apply (clarsimp split: option.splits)
+  done
+
+lemma handleInterrupt_no_fail:
+  "no_fail (ex_abs (einvs) and invs'
+                           and (\<lambda>s. intStateIRQTable (ksInterruptState s) a \<noteq> irqstate.IRQInactive))
+           (handleInterrupt a)"
+  apply (rule no_fail_pre)
+  apply (rule corres_nofail)
+    apply (rule handleInterrupt_corres)
+   apply (erule FalseE)
+  apply (fastforce simp: ex_abs_def)
+  done
+
+lemma handleEvent_Interrupt_no_fail: "no_fail (invs' and ex_abs einvs) (handleEvent Interrupt)"
+  apply (simp add: handleEvent_def)
+  apply (rule no_fail_pre)
+   apply wp
+    apply (rule handleInterrupt_no_fail)
+   apply (simp add: crunch_simps)
+   apply (rule_tac Q="\<lambda>r s. ex_abs (einvs) s \<and> invs' s \<and>
+                            (\<forall>irq. r = Some irq
+                                   \<longrightarrow> intStateIRQTable (ksInterruptState s) irq \<noteq> irqstate.IRQInactive)"
+                in hoare_strengthen_post)
+    apply (rule hoare_vcg_conj_lift)
+     apply (rule corres_ex_abs_lift)
+      apply (rule dmo_getActiveIRQ_corres)
+     apply wp
+     apply simp
     apply wp
-   apply (rule_tac Q="\<lambda>rv s. invs' s \<and> (\<forall>x. rv = Some x \<longrightarrow> x \<le> maxIRQ)
-                                     \<and> rv \<noteq> Some 0xFFFF" in hoare_post_imp)
-    apply (clarsimp simp: Kernel_C.maxIRQ_def ARM.maxIRQ_def)
-   apply (wp getActiveIRQ_le_maxIRQ getActiveIRQ_neq_Some0xFF | simp)+
+     apply simp
+    apply (rule doMachineOp_getActiveIRQ_IRQ_active)
+   apply clarsimp
   apply (clarsimp simp: invs'_def valid_state'_def)
   done
-qed
+
+end
+
+
+locale ADT_IF_Refine_1 = kernel_m +
+  fixes doUserOp_C_if ::
+    "user_transition_if \<Rightarrow> user_context \<Rightarrow> (cstate, (event option \<times> user_context)) nondet_monad"
+  assumes do_user_op_if_C_corres:
+    "corres_underlying rf_sr False False (=) (invs' and ex_abs einvs and (\<lambda>_. uop_nonempty f))
+                       \<top> (doUserOp_if f tc) (doUserOp_C_if f tc)"
+  assumes handleInterrupt_if_ccorres:
+    "ccorres (K dc \<currency> dc) (liftxf errstate id (K ()) ret__unsigned_long_') (invs') (UNIV) []
+             (handleEvent Interrupt) (handleInterruptEntry_C_body_if)"
+  and handleInvocation_ccorres':
+    "ccorres (K dc \<currency> dc) (liftxf errstate id (K ()) ret__unsigned_long_')
+       (invs' and arch_extras and ct_active' and sch_act_simple
+              and (\<lambda>s. \<forall>x. ksCurThread s \<notin> set (ksReadyQueues s x)))
+       (UNIV \<inter> {s. isCall_' s = from_bool isCall} \<inter> {s. isBlocking_' s = from_bool isBlocking}) []
+       (handleInvocation isCall isBlocking) (Call handleInvocation_'proc)"
+  and check_active_irq_corres_C:
+    "corres_underlying rf_sr False False (=) \<top> \<top> (checkActiveIRQ_if tc) (checkActiveIRQ_C_if tc)"
+  and obs_cpspace_user_data_relation:
+    "\<lbrakk> pspace_aligned' bd; pspace_distinct' bd;
+       cpspace_user_data_relation (ksPSpace bd) (underlying_memory (ksMachineState bd)) hgs \<rbrakk>
+       \<Longrightarrow> cpspace_user_data_relation (ksPSpace bd)
+             (underlying_memory (observable_memory (ksMachineState bd) (user_mem' bd))) hgs"
+begin
 
 lemma handleEvent_ccorres:
   notes K_def[simp del]
   shows
   "ccorres (\<lambda>rv rv'. (rv = Inr ()) = (rv' = scast EXCEPTION_NONE)) ret__unsigned_long_'
-           (invs' and
-               (\<lambda>s. vs_valid_duplicates' (ksPSpace s)) and
+           (invs' and arch_extras and
                 (\<lambda>s. e \<noteq> Interrupt \<longrightarrow> ct_running' s) and
                (\<lambda>s. ksSchedulerAction s = ResumeCurrentThread))
            (UNIV) []
@@ -188,59 +256,70 @@ lemma handleEvent_ccorres:
   apply (rule ccorres_guard_imp2)
    apply (simp add: handleEvent_def callKernel_C_body_if_def)
    apply (wpc, simp_all)[1]
-       apply (wpc, simp_all add: handleSyscall_C_body_if_def syscall_from_H_def liftE_def mask_def
-                                 ccorres_cond_univ_iff syscall_defs ccorres_cond_empty_iff)[1]
-              \<comment> \<open>SysCall\<close>
-              apply (simp add: handleCall_def)
-              apply (ctac (no_vcg) add: handleInvocation_ccorres)
-             \<comment> \<open>SysReplyRecv\<close>
-             apply (simp add: bind_assoc)
-             apply (rule ccorres_rhs_assoc)+
-             apply (ctac (no_vcg) add: handleReply_ccorres)
-              apply (ctac (no_vcg) add: handleRecv_ccorres)
-               apply (rule_tac P=\<top> and P'=UNIV in ccorres_from_vcg)
-               apply (rule allI, rule conseqPre, vcg)
-               apply (clarsimp simp: return_def)
-              apply wp[1]
-             apply clarsimp
-             apply wp
-             apply (rule_tac Q="\<lambda>rv s. ct_in_state' simple' s \<and> sch_act_sane s \<and>
-                                (\<forall>p. ksCurThread s \<notin> set (ksReadyQueues s p))"
-                   in hoare_post_imp)
-              apply (simp add: ct_in_state'_def)
-             apply (wp handleReply_sane handleReply_ct_not_ksQ)
+        apply (wpc; simp add: handleSyscall_C_body_if_def syscall_from_H_def
+                  ; simp add: syscall_defs liftE_def ccorres_cond_univ_iff ccorres_cond_empty_iff)
+               \<comment> \<open>SysCall\<close>
+               apply (simp add: handleCall_def)
+               apply (ctac (no_vcg) add: handleInvocation_ccorres')
+              \<comment> \<open>SysReplyRecv\<close>
+              apply (simp add: bind_assoc)
+              apply (rule ccorres_rhs_assoc)+
+              apply (ctac (no_vcg) add: handleReply_ccorres)
+               apply (ctac (no_vcg) add: handleRecv_ccorres)
+                apply (rule_tac P=\<top> and P'=UNIV in ccorres_from_vcg)
+                apply (rule allI, rule conseqPre, vcg)
+                apply (clarsimp simp: return_def)
+               apply wp[1]
+              apply clarsimp
+              apply wp
+              apply (rule_tac Q="\<lambda>rv s. ct_in_state' simple' s \<and> sch_act_sane s \<and>
+                                 (\<forall>p. ksCurThread s \<notin> set (ksReadyQueues s p))"
+                    in hoare_post_imp)
+               apply (simp add: ct_in_state'_def)
+              apply (wp handleReply_sane handleReply_ct_not_ksQ)
              \<comment> \<open>SysSend\<close>
+             apply (simp add: handleSend_def)
+             apply (ctac (no_vcg) add: handleInvocation_ccorres)
+            \<comment> \<open>SysNBSend\<close>
             apply (simp add: handleSend_def)
             apply (ctac (no_vcg) add: handleInvocation_ccorres)
-           \<comment> \<open>SysNBSend\<close>
-           apply (simp add: handleSend_def)
-           apply (ctac (no_vcg) add: handleInvocation_ccorres)
-          \<comment> \<open>SysRecv\<close>
-          apply (ctac (no_vcg) add: handleRecv_ccorres)
+           \<comment> \<open>SysRecv\<close>
+           apply (ctac (no_vcg) add: handleRecv_ccorres)
+            apply (rule_tac P=\<top> and P'=UNIV in ccorres_from_vcg)
+            apply (rule allI, rule conseqPre, vcg)
+            apply (clarsimp simp: return_def)
+           apply wp
+          \<comment> \<open>SysReply\<close>
+          apply (ctac (no_vcg) add: handleReply_ccorres)
            apply (rule_tac P=\<top> and P'=UNIV in ccorres_from_vcg)
            apply (rule allI, rule conseqPre, vcg)
            apply (clarsimp simp: return_def)
           apply wp
-         \<comment> \<open>SysReply\<close>
-         apply (ctac (no_vcg) add: handleReply_ccorres)
+         \<comment> \<open>SysYield\<close>
+         apply (ctac (no_vcg) add: handleYield_ccorres)
           apply (rule_tac P=\<top> and P'=UNIV in ccorres_from_vcg)
           apply (rule allI, rule conseqPre, vcg)
           apply (clarsimp simp: return_def)
          apply wp
-       \<comment> \<open>SysYield\<close>
-       apply (ctac (no_vcg) add: handleYield_ccorres)
-        apply (rule_tac P=\<top> and P'=UNIV in ccorres_from_vcg)
-        apply (rule allI, rule conseqPre, vcg)
-        apply (clarsimp simp: return_def)
-       apply wp
-      \<comment> \<open>SysNBRecv\<close>
-          apply (ctac (no_vcg) add: handleRecv_ccorres)
-           apply (rule_tac P=\<top> and P'=UNIV in ccorres_from_vcg)
-           apply (rule allI, rule conseqPre, vcg)
-           apply (clarsimp simp: return_def)
-          apply wp
-      \<comment> \<open>UnknownSyscall\<close>
-      apply (simp add: liftE_def bind_assoc handleUnknownSyscall_C_body_if_def)
+        \<comment> \<open>SysNBRecv\<close>
+        apply (ctac (no_vcg) add: handleRecv_ccorres)
+         apply (rule_tac P=\<top> and P'=UNIV in ccorres_from_vcg)
+         apply (rule allI, rule conseqPre, vcg)
+         apply (clarsimp simp: return_def)
+        apply wp
+       \<comment> \<open>UnknownSyscall\<close>
+       apply (simp add: liftE_def bind_assoc handleUnknownSyscall_C_body_if_def)
+       apply (rule ccorres_pre_getCurThread)
+       apply (rule ccorres_symb_exec_r)
+         apply (ctac (no_vcg) add: handleFault_ccorres)
+          apply (rule_tac P=\<top> and P'=UNIV in ccorres_from_vcg)
+          apply (rule allI, rule conseqPre, vcg)
+          apply (clarsimp simp: return_def)
+         apply wp
+        apply (clarsimp, vcg)
+       apply (clarsimp, rule conseqPre, vcg, clarsimp)
+      \<comment> \<open>UserLevelFault\<close>
+      apply (simp add: liftE_def bind_assoc handleUserLevelFault_C_body_if_def)
       apply (rule ccorres_pre_getCurThread)
       apply (rule ccorres_symb_exec_r)
         apply (ctac (no_vcg) add: handleFault_ccorres)
@@ -250,51 +329,40 @@ lemma handleEvent_ccorres:
         apply wp
        apply (clarsimp, vcg)
       apply (clarsimp, rule conseqPre, vcg, clarsimp)
-     \<comment> \<open>UserLevelFault\<close>
-     apply (simp add: liftE_def bind_assoc handleUserLevelFault_C_body_if_def)
-     apply (rule ccorres_pre_getCurThread)
-     apply (rule ccorres_symb_exec_r)
-       apply (ctac (no_vcg) add: handleFault_ccorres)
-        apply (rule_tac P=\<top> and P'=UNIV in ccorres_from_vcg)
-        apply (rule allI, rule conseqPre, vcg)
-        apply (clarsimp simp: return_def)
-       apply wp
-      apply (clarsimp, vcg)
-     apply (clarsimp, rule conseqPre, vcg, clarsimp)
-    \<comment> \<open>Interrupt\<close>
-    apply (ctac add: handleInterrupt_ccorres[unfolded handleEvent_def, simplified])
-   \<comment> \<open>VMFaultEvent\<close>
-   apply (simp add: liftE_def bind_assoc handleVMFaultEvent_C_body_if_def)
-   apply (rule ccorres_pre_getCurThread)
-   apply (simp add: catch_def)
-   apply (rule ccorres_rhs_assoc2)
-   apply (rule ccorres_split_nothrow_novcg)
-       apply (rule ccorres_split_nothrow_case_sum)
-            apply (ctac (no_vcg) add: handleVMFault_ccorres)
-           apply ceqv
+     \<comment> \<open>Interrupt\<close>
+     apply (ctac add: handleInterrupt_if_ccorres[unfolded handleEvent_def, simplified])
+    \<comment> \<open>VMFaultEvent\<close>
+    apply (simp add: liftE_def bind_assoc handleVMFaultEvent_C_body_if_def)
+    apply (rule ccorres_pre_getCurThread)
+    apply (simp add: catch_def)
+    apply (rule ccorres_rhs_assoc2)
+    apply (rule ccorres_split_nothrow_novcg)
+        apply (rule ccorres_split_nothrow_case_sum)
+             apply (ctac (no_vcg) add: handleVMFault_ccorres)
+            apply ceqv
+           apply clarsimp
           apply clarsimp
-         apply clarsimp
-         apply (rule ccorres_cond_univ)
-         apply (rule_tac P="\<lambda>s. thread = ksCurThread s" in ccorres_cross_over_guard)
-         apply (rule_tac xf'=xfdc in ccorres_call)
-            apply (ctac (no_vcg) add: handleFault_ccorres)
+          apply (rule ccorres_cond_univ)
+          apply (rule_tac P="\<lambda>s. thread = ksCurThread s" in ccorres_cross_over_guard)
+          apply (rule_tac xf'=xfdc in ccorres_call)
+             apply (ctac (no_vcg) add: handleFault_ccorres)
+            apply simp
            apply simp
           apply simp
-         apply simp
-        apply (wp hv_inv_ex')
-       apply (simp add: guard_is_UNIV_def)
-       apply (vcg exspec=handleVMFault_modifies)
-      apply ceqv
-     apply clarsimp
-     apply (rule_tac P=\<top> and P'=UNIV in ccorres_from_vcg)
-     apply (rule allI, rule conseqPre, vcg)
-     apply (clarsimp simp: return_def)
-    apply wp
-   apply (simp add: guard_is_UNIV_def)
-  apply (auto simp: ct_in_state'_def ct_not_ksQ isReply_def is_cap_fault_def
-                    cfault_rel_def seL4_Fault_UnknownSyscall_lift seL4_Fault_UserException_lift
-              elim: pred_tcb'_weakenE st_tcb_ex_cap''
-              dest: st_tcb_at_idle_thread' rf_sr_ksCurThread)
+         apply (wp hv_inv_ex')
+        apply (simp add: guard_is_UNIV_def)
+        apply (vcg exspec=handleVMFault_modifies)
+       apply ceqv
+      apply clarsimp
+      apply (rule_tac P=\<top> and P'=UNIV in ccorres_from_vcg)
+      apply (rule allI, rule conseqPre, vcg)
+      apply (clarsimp simp: return_def)
+     apply wp
+    apply (simp add: guard_is_UNIV_def)
+   apply (auto simp: ct_in_state'_def ct_not_ksQ isReply_def is_cap_fault_def
+                     cfault_rel_def seL4_Fault_UnknownSyscall_lift seL4_Fault_UserException_lift
+               elim: pred_tcb'_weakenE st_tcb_ex_cap''
+               dest: st_tcb_at_idle_thread' rf_sr_ksCurThread)
   \<comment> \<open>HypervisorEvent\<close>
   apply (simp add: liftE_def bind_assoc)
   apply (rule ccorres_guard_imp2)
@@ -308,10 +376,11 @@ lemma handleEvent_ccorres:
   done
 
 lemma kernelEntry_corres_C:
-  "corres_underlying rf_sr False False (prod_lift (\<lambda>r r'. (r = Inr ()) = (r' = Inr ()))) (
-                     all_invs' e) \<top>
-                     (kernelEntry_if e tc) (kernelEntry_C_if fp e tc)"
+  "corres_underlying rf_sr False False
+     (prod_lift (\<lambda>r r'. (r = Inr ()) = (r' = Inr ()))) (all_invs' e) \<top>
+     (kernelEntry_if e tc) (kernelEntry_C_if fp e tc)"
   using corres_nofail[OF kernel_entry_if_corres[of e tc], simplified]
+  supply nonzero_gt_zero[simp] gt_zero_nonzero[simp]
   apply (simp add: kernelEntry_if_def kernelEntry_C_if_def)
   apply (simp only: bind_assoc[symmetric])
   apply (rule corres_stateAssert_no_fail)
@@ -322,13 +391,14 @@ lemma kernelEntry_corres_C:
   apply (simp only: bind_assoc)
   apply (simp add: getCurThread_def)
   apply (rule corres_guard_imp)
-    apply (rule corres_split_deprecated [where P=\<top> and P'=\<top> and r'="\<lambda>t t'. t' = tcb_ptr_to_ctcb_ptr t"])
+    apply (rule corres_split_deprecated[where P=\<top> and P'=\<top> and r'="\<lambda>t t'. t' = tcb_ptr_to_ctcb_ptr t"])
        prefer 2
        apply (clarsimp simp: rf_sr_def cstate_relation_def Let_def)
       apply (rule corres_split_deprecated)
          prefer 2
          apply (subst archTcbUpdate_aux2[symmetric])
-         apply (rule setArchTCB_C_corres, simp, rule ccontext_rel_to_C)
+         apply (rule setTCBContext_C_corres)
+          apply (simp add: ccontext_rel_to_C)
          apply simp
         apply (rule corres_split_deprecated[OF _ ccorres_corres_u_xf, simplified bind_assoc])
             prefer 3
@@ -353,333 +423,20 @@ lemma kernelEntry_corres_C:
       apply simp
       apply (rule hoare_post_taut[where P=\<top>])
      apply wp+
-   apply (clarsimp simp: all_invs'_def invs'_def cur_tcb'_def)
-   apply fastforce
-  done
-
-end
-
-context state_rel
-begin
-
-definition
-  "ptable_rights_s'' s \<equiv> ptable_rights (cur_thread (cstate_to_A s)) (cstate_to_A s)"
-
-definition
-  "ptable_lift_s'' s \<equiv> ptable_lift (cur_thread (cstate_to_A s)) (cstate_to_A s)"
-
-definition
-  "ptable_attrs_s'' s \<equiv> ptable_attrs (cur_thread (cstate_to_A s)) (cstate_to_A s)"
-
-definition
-  "ptable_xn_s'' s \<equiv> \<lambda>addr. XNever \<in> ptable_attrs_s'' s addr"
-
-definition
-  doMachineOp_C :: "(machine_state, 'a) nondet_monad \<Rightarrow> (cstate, 'a) nondet_monad"
-where
- "doMachineOp_C mop \<equiv>
-  do
-    ms \<leftarrow> gets (\<lambda>s. phantom_machine_state_' (globals s));
-    (r, ms') \<leftarrow> select_f (mop ms);
-    modify (\<lambda>s. s \<lparr>globals := globals s \<lparr> phantom_machine_state_' := ms' \<rparr>\<rparr>);
-    return r
-  od"
-
-definition doUserOp_C_if
-  :: "user_transition_if \<Rightarrow> user_context \<Rightarrow> (cstate, (event option \<times> user_context)) nondet_monad"
-   where
-  "doUserOp_C_if uop tc \<equiv>
-   do
-      pr \<leftarrow> gets ptable_rights_s'';
-      pxn \<leftarrow> gets (\<lambda>s x. pr x \<noteq> {} \<and> ptable_xn_s'' s x);
-      pl \<leftarrow> gets (\<lambda>s. restrict_map (ptable_lift_s'' s) {x. pr x \<noteq> {}});
-      allow_read \<leftarrow> return {y. \<exists>x. pl x = Some y \<and> AllowRead \<in> pr x};
-      allow_write \<leftarrow> return {y. \<exists>x. pl x = Some y \<and> AllowWrite \<in> pr x};
-      t \<leftarrow> gets (\<lambda>s. cur_thread (cstate_to_A s));
-      um \<leftarrow> gets (\<lambda>s. user_mem_C (globals s) \<circ> ptrFromPAddr);
-      dm \<leftarrow> gets (\<lambda>s. device_mem_C (globals s) \<circ> ptrFromPAddr);
-      ds \<leftarrow> gets (\<lambda>s. device_state (phantom_machine_state_' (globals s)));
-      assert (dom (um \<circ> addrFromPPtr) \<subseteq> - dom ds);
-      assert (dom (dm \<circ> addrFromPPtr) \<subseteq> dom ds);
-      es \<leftarrow> doMachineOp_C getExMonitor;
-      u \<leftarrow> return (uop t pl pr pxn (tc, um |` allow_read, (ds \<circ> ptrFromPAddr)|` allow_read ,es));
-      assert (u \<noteq> {});
-      (e,(tc',um',ds',es')) \<leftarrow> select u;
-      setUserMem_C ((um' |` allow_write \<circ> addrFromPPtr) |` (- dom ds));
-      setDeviceState_C ((ds' |` allow_write \<circ> addrFromPPtr) |` dom ds);
-      doMachineOp_C (setExMonitor es');
-      return (e,tc')
-   od"
-
-
-definition
-  do_user_op_C_if
-  where
-  "do_user_op_C_if uop \<equiv> {(s,e,(tc,s'))| s e tc s'. ((e,tc),s') \<in> fst (split (doUserOp_C_if uop) s)}"
-
-end
-
-context kernel_m begin
-
-
-
-lemma corres_underlying_split5:
-    "(\<And>a b c d e. corres_underlying srel nf nf' rrel (Q a b c d e) (Q' a b c d e) (f a b c d e) (f' a b c d e)) \<Longrightarrow>
-     corres_underlying srel nf nf' rrel (case x of (a,b,c,d,e) \<Rightarrow> Q a b c d e) (case x of (a,b,c,d,e) \<Rightarrow> Q' a b c d e) (case x of (a,b,c,d,e) \<Rightarrow> f a b c d e) (case x of (a,b,c,d,e) \<Rightarrow> f' a b c d e)"
-  apply (case_tac x)
-  apply simp
-  done
-
-lemma corres_select_f':
-  "\<lbrakk> \<And>s s'. P s \<Longrightarrow> P' s' \<Longrightarrow> \<forall>s' \<in> fst S'. \<exists>s \<in> fst S. rvr s s'; nf' \<Longrightarrow> \<not> snd S' \<rbrakk>
-      \<Longrightarrow> corres_underlying sr nf nf' rvr P P' (select_f S) (select_f S')"
-  by (clarsimp simp: select_f_def corres_underlying_def)
-
-lemma corres_dmo_getExMonitor_C:
-  "corres_underlying rf_sr nf nf' (=) \<top> \<top> (doMachineOp getExMonitor) (doMachineOp_C getExMonitor)"
-  supply subst_all [simp del]
-  apply (clarsimp simp: doMachineOp_def doMachineOp_C_def)
-  apply (rule corres_guard_imp)
-    apply (rule_tac r'="\<lambda>ms ms'. exclusive_state ms = exclusive_state ms' \<and> machine_state_rest ms = machine_state_rest ms'
-      \<and> irq_masks ms = irq_masks ms' \<and> equiv_irq_state ms ms' \<and> device_state ms = device_state ms'" and P="\<top>" and P'="\<top>" in corres_split_deprecated)
-       apply (rule_tac r'="\<lambda>(r, ms) (r', ms'). r = r' \<and> ms = rv \<and> ms' = rv'" in corres_split_deprecated)
-          apply (clarsimp simp: split_def)
-          apply (rule_tac r'=dc and P="\<lambda>s. underlying_memory (snd ((aa, bb), ba)) = underlying_memory (ksMachineState s)"
-                 and P'="\<lambda>s. underlying_memory (snd ((aa, bb), bc)) = underlying_memory (phantom_machine_state_' (globals s))" in corres_split_deprecated)
-             apply clarsimp
-            apply (rule corres_modify)
-            apply (clarsimp simp: rf_sr_def cstate_relation_def carch_state_relation_def cmachine_state_relation_def Let_def)
-           apply (wp hoare_TrueI)+
-         apply (rule corres_select_f')
-          apply (clarsimp simp: getExMonitor_def machine_rest_lift_def NonDetMonad.bind_def gets_def get_def return_def modify_def put_def select_f_def)
-         apply (clarsimp simp: getExMonitor_no_fail[simplified no_fail_def])
-        apply (wp hoare_TrueI)+
-      apply (clarsimp simp: rf_sr_def cstate_relation_def cmachine_state_relation_def Let_def)
-     apply (wp hoare_TrueI)+
-  apply (rule TrueI conjI | clarsimp simp: getExMonitor_def machine_rest_lift_def NonDetMonad.bind_def gets_def get_def return_def modify_def put_def select_f_def)+
-  done
-
-lemma corres_dmo_setExMonitor_C:
-  "corres_underlying rf_sr nf nf' dc \<top> \<top> (doMachineOp (setExMonitor es)) (doMachineOp_C (setExMonitor es))"
-  apply (clarsimp simp: doMachineOp_def doMachineOp_C_def)
-  apply (rule corres_guard_imp)
-    apply (rule_tac r'="\<lambda>ms ms'. exclusive_state ms = exclusive_state ms' \<and> machine_state_rest ms = machine_state_rest ms'
-      \<and> irq_masks ms = irq_masks ms' \<and> equiv_irq_state ms ms' \<and> device_state ms = device_state ms'" and P="\<top>" and P'="\<top>" in corres_split_deprecated)
-       apply (rule_tac r'="\<lambda>(r, ms) (r', ms'). ms = rv\<lparr>exclusive_state := es\<rparr> \<and> ms' = rv'\<lparr>exclusive_state := es\<rparr>" in corres_split_deprecated)
-          apply (simp add: split_def)
-          apply (rule_tac P="\<lambda>s. underlying_memory (snd rva) = underlying_memory (ksMachineState s)"
-                 and P'="\<lambda>s. underlying_memory (snd rv'a) = underlying_memory (phantom_machine_state_' (globals s))" in corres_modify)
-          apply (clarsimp simp: rf_sr_def cstate_relation_def carch_state_relation_def cmachine_state_relation_def Let_def)
-         apply (rule corres_select_f')
-          apply (clarsimp simp: setExMonitor_def machine_rest_lift_def NonDetMonad.bind_def gets_def get_def return_def modify_def put_def select_f_def)
-         apply (clarsimp simp: setExMonitor_no_fail[simplified no_fail_def])
-        apply (wp hoare_TrueI)+
-      apply (clarsimp simp: rf_sr_def cstate_relation_def cmachine_state_relation_def Let_def)
-     apply (wp hoare_TrueI)+
-  apply (rule TrueI conjI | clarsimp simp: setExMonitor_def machine_rest_lift_def NonDetMonad.bind_def gets_def get_def return_def modify_def put_def select_f_def)+
-  done
-
-lemma dmo_getExMonitor_C_wp[wp]:
-  "\<lbrace>\<lambda>s. P (exclusive_state (phantom_machine_state_' (globals s))) s\<rbrace>
-   doMachineOp_C getExMonitor \<lbrace>P\<rbrace>"
-  apply(simp add: doMachineOp_C_def)
-  apply(wp modify_wp | wpc)+
-  apply clarsimp
-  apply(erule use_valid)
-   apply wp
-  apply simp
-  done
-
-lemma cur_thread_of_absKState[simp]:
-   "cur_thread (absKState s) = (ksCurThread s)"
-   by (clarsimp simp: cstate_relation_def Let_def absKState_def cstate_to_H_def)
-
-lemma absKState_crelation:
-  "\<lbrakk>cstate_relation s (globals s'); invs' s\<rbrakk>\<Longrightarrow>  cstate_to_A s' = absKState s"
-  apply (clarsimp simp add: cstate_to_H_correct invs'_def cstate_to_A_def)
-  apply (clarsimp simp: absKState_def absExst_def observable_memory_def)
-  apply (case_tac s)
-  apply clarsimp
-  apply (case_tac ksMachineState)
-  apply clarsimp
-  apply (rule ext)
-  by (clarsimp simp: option_to_0_def user_mem'_def pointerInUserData_def ko_wp_at'_def
-                     obj_at'_def typ_at'_def ps_clear_def
-              split: if_splits)
-
-lemma do_user_op_if_C_corres:
-   "corres_underlying rf_sr False False (=)
-   (invs' and ex_abs einvs and (\<lambda>_. uop_nonempty f)) \<top>
-   (doUserOp_if f tc) (doUserOp_C_if f tc)"
-  apply (rule corres_gen_asm)
-  apply (simp add: doUserOp_if_def doUserOp_C_if_def uop_nonempty_def del: split_paired_All)
-  apply (rule corres_gets_same)
-    apply (clarsimp simp: absKState_crelation ptable_rights_s'_def ptable_rights_s''_def
-           rf_sr_def  cstate_relation_def Let_def cstate_to_H_correct)
-   apply simp
-  apply (rule corres_gets_same)
-    apply (clarsimp simp: ptable_xn_s'_def ptable_xn_s''_def ptable_attrs_s_def
-                          absKState_crelation ptable_attrs_s'_def ptable_attrs_s''_def  rf_sr_def)
-   apply simp
-  apply (rule corres_gets_same)
-    apply (clarsimp simp: absKState_crelation curthread_relation ptable_lift_s'_def ptable_lift_s''_def
-                         ptable_lift_s_def rf_sr_def)
-   apply simp
-  apply (simp add: getCurThread_def)
-  apply (rule corres_gets_same)
-    apply (simp add: absKState_crelation rf_sr_def)
-   apply simp
-  apply (rule corres_gets_same)
-    apply (rule fun_cong[where x=ptrFromPAddr])
-    apply (rule_tac f=comp in arg_cong)
-    apply (rule user_mem_C_relation[symmetric])
-    apply (simp add: rf_sr_def cstate_relation_def Let_def
-                               cpspace_relation_def)
-    apply fastforce
-   apply simp
-  apply (rule corres_gets_same)
-    apply (clarsimp simp: rf_sr_def cstate_relation_def Let_def
-                          cpspace_relation_def)
-    apply (drule device_mem_C_relation[symmetric])
-     apply fastforce
-    apply (simp add: comp_def)
-   apply simp
-  apply (rule corres_gets_same)
-    apply (clarsimp simp: cstate_relation_def rf_sr_def
-                          Let_def cmachine_state_relation_def)
-   apply simp
-  apply (rule corres_guard_imp)
-    apply (rule_tac P=\<top> and P'=\<top> and r'="(=)" in corres_split_deprecated)
-       prefer 2
-       apply (clarsimp simp add: corres_underlying_def fail_def
-                                 assert_def return_def
-                          split: if_splits)
-      apply simp
-      apply (rule_tac P=\<top> and P'=\<top> and r'="(=)" in corres_split_deprecated)
-         prefer 2
-         apply (clarsimp simp add: corres_underlying_def fail_def
-                                   assert_def return_def
-                            split: if_splits)
-        apply simp
-        apply (rule corres_split_deprecated[OF _ corres_dmo_getExMonitor_C])
-          apply clarsimp
-          apply (rule_tac r'="(=)" in corres_split_deprecated[OF _ corres_select])
-              prefer 2
-              apply clarsimp
-             apply simp
-             apply (rule corres_underlying_split5)
-             apply (rule corres_split_deprecated[OF _ user_memory_update_corres_C])
-               apply (rule corres_split_deprecated[OF _ device_update_corres_C])
-                 apply (rule corres_split_deprecated[OF _ corres_dmo_setExMonitor_C,
-                               where R="\<top>\<top>" and R'="\<top>\<top>"])
-                        apply (wp select_wp | simp)+
-    apply (clarsimp simp:  ex_abs_def restrict_map_def invs_pspace_aligned'
-                           invs_pspace_distinct' ptable_lift_s'_def ptable_rights_s'_def
-                   split: if_splits)
-    apply (drule ptable_rights_imp_UserData[rotated -1])
-     apply ((fastforce | intro conjI)+)[4]
-    apply (clarsimp simp: user_mem'_def device_mem'_def dom_def split: if_splits)
-    apply fastforce
-   apply (clarsimp simp add: invs'_def valid_state'_def valid_pspace'_def ex_abs_def)
-   done
-
-definition
-  checkActiveIRQ_C_if :: "user_context \<Rightarrow> (cstate, irq option \<times> user_context) nondet_monad"
-  where
-  "checkActiveIRQ_C_if tc \<equiv>
-   do
-      getActiveIRQ_C;
-      irq \<leftarrow>  gets ret__unsigned_long_';
-      return (if irq = 0xFFFF then None else Some (ucast irq), tc)
-   od"
-
-definition
-  check_active_irq_C_if
-  where
-  "check_active_irq_C_if \<equiv> {((tc, s), irq, (tc', s')). ((irq, tc'), s') \<in> fst (checkActiveIRQ_C_if tc s)}"
-
-lemma check_active_irq_corres_C:
-  "corres_underlying rf_sr False False (=) \<top> \<top>
-                     (checkActiveIRQ_if tc) (checkActiveIRQ_C_if tc)"
-  apply (simp add: checkActiveIRQ_if_def checkActiveIRQ_C_if_def)
-  apply (simp add: getActiveIRQ_C_def)
-  apply (subst bind_assoc[symmetric])
-  apply (rule corres_guard_imp)
-    apply (rule corres_split_deprecated[where r'="\<lambda>a c. case a of None \<Rightarrow> c = 0xFFFF | Some x \<Rightarrow> c = ucast x \<and> c \<noteq> 0xFFFF", OF _ ccorres_corres_u_xf])
-        apply (clarsimp split: if_split option.splits)
-       apply (rule ccorres_guard_imp)
-         apply (rule ccorres_rel_imp, rule ccorres_guard_imp)
-            apply (rule getActiveIRQ_ccorres)
-           apply simp+
-         apply (case_tac x; simp add: ucast_helper_simps_32)
-        apply simp+
-      apply (rule no_fail_dmo')
-      apply (rule getActiveIRQ_nf)
-     apply (rule hoare_post_taut[where P=\<top>])+
-   apply simp+
-   apply fastforce
-  done
-
-
-definition
-  handlePreemption_C_if :: "user_context \<Rightarrow> (cstate,user_context) nondet_monad" where
-  "handlePreemption_C_if tc \<equiv>
-       do (exec_C \<Gamma> handleInterruptEntry_C_body_if); return tc od"
-
-lemma handlePreemption_if_def2:
-  "handlePreemption_if tc = do
-     r \<leftarrow> handleEvent Interrupt;
-          stateAssert (\<lambda>s. (ksDomainTime s = 0 \<longrightarrow> ksSchedulerAction s = ChooseNewThread) \<and>
-                            valid_domain_list' s) [];
-          return tc
-   od"
-  apply (clarsimp simp add: handlePreemption_if_def handleEvent_def liftE_def
-                   bind_assoc)
-  apply (rule bind_eqI)
-  apply (rule ext)
-  apply (clarsimp split: option.splits)
-  done
-
-lemma handleInterrupt_no_fail: "no_fail (ex_abs (einvs) and invs' and (\<lambda>s. intStateIRQTable (ksInterruptState s) a \<noteq> irqstate.IRQInactive)) (handleInterrupt a)"
-  apply (rule no_fail_pre)
-  apply (rule corres_nofail)
-    apply (rule handleInterrupt_corres)
-   apply (erule FalseE)
-  apply (fastforce simp: ex_abs_def)
-  done
-
-lemma handleEvent_Interrupt_no_fail: "no_fail (invs' and ex_abs einvs) (handleEvent Interrupt)"
-  apply (simp add: handleEvent_def)
-  apply (rule no_fail_pre)
-   apply wp
-    apply (rule handleInterrupt_no_fail)
-   apply (simp add: crunch_simps)
-   apply (rule_tac Q="\<lambda>r s. ex_abs (einvs) s \<and>
-                      invs' s \<and> (\<forall>irq. r = Some irq \<longrightarrow> intStateIRQTable (ksInterruptState s) irq \<noteq> irqstate.IRQInactive)" in hoare_strengthen_post)
-    apply (rule hoare_vcg_conj_lift)
-     apply (rule corres_ex_abs_lift)
-      apply (rule dmo_getActiveIRQ_corres)
-     apply wp
-     apply simp
-    apply wp
-     apply simp
-    apply (rule doMachineOp_getActiveIRQ_IRQ_active)
-   apply clarsimp
-  apply (clarsimp simp: invs'_def valid_state'_def)
+   apply (clarsimp simp: all_invs'_def invs'_def cur_tcb'_def valid_state'_def)
+  apply fastforce
   done
 
 lemma handle_preemption_corres_C:
   "corres_underlying rf_sr False False (=)
-                     (invs' and (\<lambda>s. vs_valid_duplicates' (ksPSpace s)) and
-                      valid_domain_list' and (\<lambda>s. 0 < ksDomainTime s) and
-                      ex_abs einvs) \<top>
-                     (handlePreemption_if tc) (handlePreemption_C_if tc)"
+     (invs' and valid_domain_list' and (\<lambda>s. 0 < ksDomainTime s) and ex_abs einvs) \<top>
+     (handlePreemption_if tc) (handlePreemption_C_if tc)"
   apply (simp add: handlePreemption_if_def2 handlePreemption_C_if_def)
   apply (rule corres_stateAssert_no_fail)
    using corres_nofail[OF handle_preemption_if_corres[of tc], simplified]
    apply (simp add: handlePreemption_if_def2)
    apply (erule no_fail_pre)
-   apply (clarsimp simp: ex_abs_underlying_def)
+   apply (clarsimp simp: ex_abs_underlying_def ex_abs_def)
    apply (rule exI, rule conjI, assumption)
    apply (clarsimp simp: domain_time_rel_eq domain_list_rel_eq)
   apply (rule corres_guard_imp)
@@ -688,7 +445,7 @@ lemma handle_preemption_corres_C:
       apply (rule ccorres_corres_u)
        apply (rule ccorres_guard_imp)
          apply (rule ccorres_rel_imp)
-          apply (rule handleInterrupt_ccorres)
+          apply (rule handleInterrupt_if_ccorres)
          apply simp
         prefer 3
         apply (rule handleEvent_Interrupt_no_fail)
@@ -698,24 +455,25 @@ lemma handle_preemption_corres_C:
    apply (fastforce simp: ex_abs_def schedaction_related)+
   done
 
+end
+
+
+context kernel_m begin
 
 definition
   handle_preemption_C_if
   where
   "handle_preemption_C_if \<equiv>
-      {(s, u, s'). s' \<in> fst (split handlePreemption_C_if s)}"
+     {(s, u, s'). s' \<in> fst (split handlePreemption_C_if s)}"
 
 definition
   schedule_C_if' :: "user_context \<Rightarrow> (cstate,user_context) nondet_monad" where
   "schedule_C_if' tc \<equiv>
-    do exec_C \<Gamma> (Call schedule_'proc); exec_C \<Gamma> (Call activateThread_'proc); return tc od"
-
+     do exec_C \<Gamma> (Call schedule_'proc); exec_C \<Gamma> (Call activateThread_'proc); return tc od"
 
 lemma ccorres_corres_u':
-  "\<lbrakk>ccorres dc xfdc P' Q' [] H C; no_fail P'' H;
-    (\<And>s. P s \<Longrightarrow> P' s \<and> P'' s);
-    (Collect Q) \<subseteq> Q'\<rbrakk> \<Longrightarrow>
-   corres_underlying rf_sr nf nf' dc P Q H (exec_C \<Gamma> C)"
+  "\<lbrakk> ccorres dc xfdc P' Q' [] H C; no_fail P'' H; (\<And>s. P s \<Longrightarrow> P' s \<and> P'' s); (Collect Q) \<subseteq> Q' \<rbrakk>
+     \<Longrightarrow> corres_underlying rf_sr nf nf' dc P Q H (exec_C \<Gamma> C)"
   apply (rule ccorres_corres_u)
    apply (rule ccorres_guard_imp)
      apply assumption
@@ -724,12 +482,11 @@ lemma ccorres_corres_u':
   apply (rule no_fail_pre,simp+)
   done
 
-
 lemma schedule_if_corres_C:
   "corres_underlying rf_sr False False (=)
-                     (invs' and ex_abs einvs and valid_domain_list' and
-                      (\<lambda>s. ksDomainTime s = 0 \<longrightarrow> ksSchedulerAction s = ChooseNewThread)) \<top>
-                     (schedule'_if tc) (schedule_C_if' tc)"
+     (invs' and ex_abs einvs and valid_domain_list'
+            and (\<lambda>s. ksDomainTime s = 0 \<longrightarrow> ksSchedulerAction s = ChooseNewThread)) \<top>
+     (schedule'_if tc) (schedule_C_if' tc)"
   apply (simp add: schedule'_if_def schedule_C_if'_def)
   apply (subst bind_assoc[symmetric], rule corres_stateAssert_no_fail)
    using corres_nofail[OF schedule_if_corres[of tc], simplified]
@@ -760,7 +517,8 @@ lemma schedule_if_corres_C:
         apply (erule FalseE)
        apply simp
       apply simp
-     apply (rule_tac Q="\<lambda>r. ct_in_state' activatable' and invs' and ex_abs(invs and ct_in_state activatable)" in hoare_strengthen_post)
+     apply (rule_tac Q="\<lambda>r. ct_in_state' activatable' and invs' and
+                            ex_abs (invs and ct_in_state activatable)" in hoare_strengthen_post)
       apply (wp schedule_invs' corres_ex_abs_lift)
        apply (rule schedule_corres)
       apply wp
@@ -771,26 +529,44 @@ lemma schedule_if_corres_C:
    apply (auto simp: ex_abs_def)
   done
 
-definition
-  schedule_C_if
-  where
-  "schedule_C_if \<equiv>
-      {(s, (e :: unit), s'). s' \<in> fst (split schedule_C_if' s)}"
 
-definition
- kernelExit_C_if :: "user_context \<Rightarrow> (cstate,user_context) nondet_monad" where
+definition schedule_C_if where
+  "schedule_C_if \<equiv> {(s, (e :: unit), s'). s' \<in> fst (split schedule_C_if' s)}"
+
+definition kernelExit_C_if :: "user_context \<Rightarrow> (cstate,user_context) nondet_monad" where
   "kernelExit_C_if tc \<equiv>
    do t \<leftarrow> gets (ksCurThread_' \<circ> globals);
       gets $ getContext_C t
    od"
 
+definition kernel_exit_C_if where
+  "kernel_exit_C_if \<equiv>
+     {(s, m, s'). s' \<in> fst (split kernelExit_C_if s) \<and>
+                  m = (if ct_running_C (snd s') then InUserMode else InIdleMode)}"
+
+end
+
+
 lemma corres_underlying_nf_imp2:
   "corres_underlying rf_sr nf True a b c d e \<Longrightarrow> corres_underlying rf_sr nf nf' a b c d e"
   by (auto simp: corres_underlying_def)
 
+lemma preserves_trivial: "preserves mode mode' UNIV f"
+  apply (simp add: preserves_def)
+  done
+
+lemma preserves'_trivial: "preserves' mode UNIV f"
+  apply (simp add: preserves'_def)
+  done
+
+
+context ADT_IF_Refine_1 begin
+
+definition do_user_op_C_if where
+  "do_user_op_C_if uop \<equiv> {(s,e,(tc,s'))| s e tc s'. ((e,tc),s') \<in> fst (split (doUserOp_C_if uop) s)}"
+
 lemma kernel_exit_corres_C:
-  "corres_underlying rf_sr False nf (=) (invs') \<top>
-                     (kernelExit_if tc) (kernelExit_C_if tc)"
+  "corres_underlying rf_sr False nf (=) (invs') \<top> (kernelExit_if tc) (kernelExit_C_if tc)"
   apply (rule corres_underlying_nf_imp2)
   apply (simp add: kernelExit_if_def kernelExit_C_if_def)
   apply (rule corres_guard_imp)
@@ -804,35 +580,6 @@ lemma kernel_exit_corres_C:
    apply clarsimp+
   done
 
-
-definition
-  kernel_exit_C_if
-  where
-  "kernel_exit_C_if \<equiv>
-      {(s, m, s'). s' \<in> fst (split kernelExit_C_if s) \<and>
-                   m = (if ct_running_C (snd s') then InUserMode else InIdleMode)}"
-
-end
-
-lemma preserves_trivial: "preserves mode mode' UNIV f"
-  apply (simp add: preserves_def)
-  done
-
-lemma preserves'_trivial: "preserves' mode UNIV f"
-  apply (simp add: preserves'_def)
-  done
-
-context kernel_m begin
-
-
-definition ADT_C_if where
-"ADT_C_if fp uop \<equiv> \<lparr>Init = \<lambda>s. ({user_context_of s} \<times> {s'. cstate_to_A s' = (internal_state_if s)}) \<times> {sys_mode_of s} \<inter> {s''. \<exists>s'. ((internal_state_if s'),(internal_state_if s'')) \<in> rf_sr \<and> s' \<in> full_invs_if' \<and> sys_mode_of s = sys_mode_of s'},
-                  Fin = \<lambda>((uc,s),m). ((uc, cstate_to_A s),m),
-                  Step = (\<lambda>(u :: unit). global_automaton_if
-                              check_active_irq_C_if (do_user_op_C_if uop)
-                              (kernel_call_C_if fp) handle_preemption_C_if
-                              schedule_C_if kernel_exit_C_if)\<rparr>"
-
 lemma full_invs_all_invs[simp]:
   "((tc,s),KernelEntry e) \<in> full_invs_if' \<Longrightarrow> all_invs' e s"
   apply (clarsimp simp: full_invs_if'_def all_invs'_def ex_abs_def)
@@ -840,44 +587,11 @@ lemma full_invs_all_invs[simp]:
   by (auto simp: ct_running_related ct_idle_related schedaction_related
                  domain_time_rel_eq domain_list_rel_eq)
 
-lemma obs_cpspace_user_data_relation:
-  "\<lbrakk>pspace_aligned' bd;pspace_distinct' bd;
-    cpspace_user_data_relation (ksPSpace bd) (underlying_memory (ksMachineState bd)) hgs\<rbrakk>
-   \<Longrightarrow> cpspace_user_data_relation (ksPSpace bd) (underlying_memory (observable_memory (ksMachineState bd) (user_mem' bd))) hgs"
-   apply (clarsimp simp: cmap_relation_def dom_heap_to_user_data)
-   apply (drule bspec,fastforce)
-   apply (clarsimp simp: cuser_user_data_relation_def observable_memory_def
-                         heap_to_user_data_def map_comp_def Let_def
-                  split: option.split_asm)
-   apply (drule_tac x = off in spec)
-   apply (subst option_to_0_user_mem')
-   apply (subst map_option_byte_to_word_heap)
-    apply (clarsimp simp: projectKO_opt_user_data pointerInUserData_def field_simps
-                   split: kernel_object.split_asm option.split_asm)
-    apply (frule(1) pspace_alignedD')
-    apply (subst neg_mask_add_aligned)
-      apply (simp add: objBits_simps)
-     apply (simp add: word_less_nat_alt)
-     apply (rule le_less_trans[OF unat_plus_gt])
-     apply (subst add.commute)
-     apply (subst unat_mult_simple)
-      apply (simp add: word_bits_def)
-      apply (rule less_le_trans[OF unat_lt2p])
-      apply simp
-     apply simp
-    apply (rule nat_add_offset_less [where n = 2, simplified])
-      apply simp
-     apply (rule unat_lt2p)
-    apply (simp add: pageBits_def objBits_simps)
-   apply (frule(1) pspace_distinctD')
-   apply (clarsimp simp: obj_at'_def typ_at'_def ko_wp_at'_def objBits_simps)
-  apply simp
-  done
-
 lemma obs_cpspace_device_data_relation:
-  "\<lbrakk>pspace_aligned' bd;pspace_distinct' bd;
-    cpspace_device_data_relation (ksPSpace bd) (underlying_memory (ksMachineState bd)) hgs\<rbrakk>
-   \<Longrightarrow> cpspace_device_data_relation (ksPSpace bd) (underlying_memory (observable_memory (ksMachineState bd) (user_mem' bd))) hgs"
+  "\<lbrakk> pspace_aligned' bd; pspace_distinct' bd;
+     cpspace_device_data_relation (ksPSpace bd) (underlying_memory (ksMachineState bd)) hgs \<rbrakk>
+     \<Longrightarrow> cpspace_device_data_relation (ksPSpace bd)
+           (underlying_memory (observable_memory (ksMachineState bd) (user_mem' bd))) hgs"
    apply (clarsimp simp: cmap_relation_def dom_heap_to_device_data)
    apply (drule bspec,fastforce)
    apply (clarsimp simp: cuser_user_data_device_relation_def observable_memory_def
@@ -886,21 +600,32 @@ lemma obs_cpspace_device_data_relation:
    done
 
 lemma cstate_relation_observable_memory:
-  "\<lbrakk>invs' bs;cstate_relation bs gs\<rbrakk>
-  \<Longrightarrow> cstate_relation (bs\<lparr>ksMachineState := observable_memory (ksMachineState bs) (user_mem' bs)\<rparr>) gs"
+  "\<lbrakk> invs' bs; cstate_relation bs gs \<rbrakk>
+     \<Longrightarrow> cstate_relation (bs\<lparr>ksMachineState := observable_memory (ksMachineState bs) (user_mem' bs)\<rparr>) gs"
   by (clarsimp simp: cstate_relation_def Let_def obs_cpspace_user_data_relation
                      obs_cpspace_device_data_relation cpspace_relation_def invs'_def
                      valid_state'_def valid_pspace'_def
                      cmachine_state_relation_def observable_memory_def)
 
 
+definition ADT_C_if where
+  "ADT_C_if fp uop \<equiv>
+     \<lparr>Init = \<lambda>s. ({user_context_of s} \<times> {s'. cstate_to_A s' = (internal_state_if s)}) \<times>
+                  {sys_mode_of s} \<inter> {s''. \<exists>s'. ((internal_state_if s'),(internal_state_if s'')) \<in> rf_sr \<and>
+                                                s' \<in> full_invs_if' \<and> sys_mode_of s = sys_mode_of s'},
+                  Fin = \<lambda>((uc,s),m). ((uc, cstate_to_A s),m),
+                  Step = (\<lambda>(u :: unit). global_automaton_if
+                              check_active_irq_C_if (do_user_op_C_if uop)
+                              (kernel_call_C_if fp) handle_preemption_C_if
+                              schedule_C_if kernel_exit_C_if)\<rparr>"
+
+
 lemma c_to_haskell:
-  "uop_nonempty uop \<Longrightarrow>
-   global_automata_refine checkActiveIRQ_H_if (doUserOp_H_if uop) kernelCall_H_if
-     handlePreemption_H_if schedule'_H_if kernelExit_H_if full_invs_if' (ADT_H_if uop) UNIV
-     check_active_irq_C_if (do_user_op_C_if uop) (kernel_call_C_if fp) handle_preemption_C_if schedule_C_if
-     kernel_exit_C_if UNIV (ADT_C_if fp uop) (lift_snd_rel rf_sr) False"
-  supply subst_all [simp del]
+  "uop_nonempty uop
+   \<Longrightarrow> global_automata_refine checkActiveIRQ_H_if (doUserOp_H_if uop) kernelCall_H_if
+         handlePreemption_H_if schedule'_H_if kernelExit_H_if full_invs_if' (ADT_H_if uop) UNIV
+         check_active_irq_C_if (do_user_op_C_if uop) (kernel_call_C_if fp) handle_preemption_C_if
+         schedule_C_if kernel_exit_C_if UNIV (ADT_C_if fp uop) (lift_snd_rel rf_sr) False"
   apply (simp add: global_automata_refine_def)
   apply (intro conjI)
     apply (rule haskell_invs)
@@ -913,7 +638,7 @@ lemma c_to_haskell:
          apply (simp add: ADT_H_if_def ADT_C_if_def lift_fst_rel_def lift_snd_rel_def)
          apply safe
          apply (clarsimp simp: absKState_crelation  rf_sr_def full_invs_if'_def)
-         apply (rule_tac x="((a,bd),ba)" in bexI)
+         apply (rule_tac x="((a,bb),ba)" in bexI)
           apply simp
          apply simp
          apply (frule cstate_to_H_correct[rotated],simp add: invs'_def)
@@ -964,6 +689,5 @@ theorem infoflow_refinement_A: "uop_nonempty uop \<Longrightarrow> ADT_C_if fp u
   done
 
 end
-
 
 end
