proof/crefine/ARM/ADT_C.thy
@@ -55,10 +55,11 @@ definition
    else callKernel_C e"
 
 definition
-  setArchTCB_C :: "arch_tcb_C \<Rightarrow> tcb_C ptr \<Rightarrow> (cstate,unit) nondet_monad"
+  setTCBContext_C :: "user_context_C \<Rightarrow> tcb_C ptr \<Rightarrow> (cstate,unit) nondet_monad"
 where
-  "setArchTCB_C ct thread \<equiv>
-  exec_C \<Gamma> (\<acute>t_hrs :== hrs_mem_update (heap_update (Ptr &(thread\<rightarrow>[''tcbArch_C''])) ct) \<acute>t_hrs)"
+  "setTCBContext_C ct thread \<equiv>
+  exec_C \<Gamma> (\<acute>t_hrs :== hrs_mem_update (heap_update (
+    Ptr &((Ptr &(thread\<rightarrow>[''tcbArch_C'']) :: (arch_tcb_C ptr))\<rightarrow>[''tcbContext_C''])) ct) \<acute>t_hrs)"
 
 lemma Basic_sem_eq:
   "\<Gamma>\<turnstile>\<langle>Basic f,s\<rangle> \<Rightarrow> s' = ((\<exists>t. s = Normal t \<and> s' = Normal (f t)) \<or> (\<forall>t. s \<noteq> Normal t \<and> s' = s))"
@@ -72,14 +73,14 @@ lemma Basic_sem_eq:
   apply (cases s, auto)
   done
 
-lemma setArchTCB_C_corres:
-  "\<lbrakk> ccontext_relation tc (tcbContext_C tc'); t' = tcb_ptr_to_ctcb_ptr t \<rbrakk> \<Longrightarrow>
-  corres_underlying rf_sr nf nf' dc (tcb_at' t) \<top>
-    (threadSet (\<lambda>tcb. tcb \<lparr> tcbArch := atcbContextSet tc (tcbArch tcb)\<rparr>) t) (setArchTCB_C tc' t')"
-  apply (simp add: setArchTCB_C_def exec_C_def Basic_sem_eq corres_underlying_def)
+lemma setTCBContext_C_corres:
+  "\<lbrakk> ccontext_relation tc tc'; t' = tcb_ptr_to_ctcb_ptr t \<rbrakk> \<Longrightarrow>
+  corres_underlying rf_sr nf nf' dc (pspace_domain_valid and tcb_at' t) \<top>
+    (threadSet (\<lambda>tcb. tcb \<lparr> tcbArch := atcbContextSet tc (tcbArch tcb)\<rparr>) t) (setTCBContext_C tc' t')"
+  apply (simp add: setTCBContext_C_def exec_C_def Basic_sem_eq corres_underlying_def)
   apply clarsimp
   apply (simp add: threadSet_def bind_assoc split_def exec_gets)
-  apply (drule (1) obj_at_cslift_tcb)
+  apply (frule (1) obj_at_cslift_tcb)
   apply clarsimp
   apply (frule getObject_eq [rotated -1], simp)
    apply (simp add: objBits_simps')
@@ -102,13 +103,10 @@ lemma setArchTCB_C_corres:
                         carch_state_relation_def cmachine_state_relation_def
                         typ_heap_simps' update_tcb_map_tos)
   apply (simp add: map_to_ctes_upd_tcb_no_ctes map_to_tcbs_upd tcb_cte_cases_def
-                   cvariable_relation_upd_const ko_at_projectKO_opt)
+                   cvariable_relation_upd_const ko_at_projectKO_opt cteSizeBits_def)
   apply (simp add: cep_relations_drop_fun_upd)
-  apply (rule conjI)
-   defer
-   apply (erule cready_queues_relation_not_queue_ptrs)
-    apply (rule ext, simp split: if_split)
-   apply (rule ext, simp split: if_split)
+  apply (apply_conjunct \<open>match conclusion in \<open>cready_queues_relation _ _ _\<close> \<Rightarrow>
+         \<open>erule cready_queues_relation_not_queue_ptrs; rule ext; simp split: if_split\<close>\<close>)
   apply (drule ko_at_projectKO_opt)
   apply (erule (2) cmap_relation_upd_relI)
     apply (simp add: ctcb_relation_def carch_tcb_relation_def)
@@ -159,7 +157,7 @@ definition
   where
   "kernelEntry_C fp e tc \<equiv> do
     t \<leftarrow> gets (ksCurThread_' o globals);
-    setArchTCB_C (arch_tcb_C (to_user_context_C tc)) t;
+    setTCBContext_C (to_user_context_C tc) t;
     if fp then callKernel_withFastpath_C e else callKernel_C e;
     t \<leftarrow> gets (ksCurThread_' o globals);
     gets $ getContext_C t
@@ -1515,15 +1513,16 @@ definition
    else callKernel_C e"
 
 definition
-  setArchTCB_C :: "arch_tcb_C \<Rightarrow> tcb_C ptr \<Rightarrow> (cstate,unit) nondet_monad"
+  setTCBContext_C :: "user_context_C \<Rightarrow> tcb_C ptr \<Rightarrow> (cstate,unit) nondet_monad"
 where
-  "setArchTCB_C ct thread \<equiv>
-  exec_C \<Gamma> (\<acute>t_hrs :== hrs_mem_update (heap_update (Ptr &(thread\<rightarrow>[''tcbArch_C''])) ct) \<acute>t_hrs)"
+  "setTCBContext_C ct thread \<equiv>
+  exec_C \<Gamma> (\<acute>t_hrs :== hrs_mem_update (heap_update (
+    Ptr &((Ptr &(thread\<rightarrow>[''tcbArch_C'']) :: (arch_tcb_C ptr))\<rightarrow>[''tcbContext_C''])) ct) \<acute>t_hrs)"
 
 definition
   "kernelEntry_C fp e tc \<equiv> do
     t \<leftarrow> gets (ksCurThread_' o globals);
-    setArchTCB_C (arch_tcb_C (to_user_context_C tc)) t;
+    setTCBContext_C (to_user_context_C tc) t;
     if fp then callKernel_withFastpath_C e else callKernel_C e;
     t \<leftarrow> gets (ksCurThread_' o globals);
     gets $ getContext_C t
